scratching around

interface_abstraction/Scratch.thy
@@ -33,292 +33,163 @@ lemma fixes G::"'v graph" and Gafp::"('v, 'v \<times> 'v) pre_digraph"
 definition pcycle :: "'v set \<Rightarrow> ('v \<times> 'v) set \<Rightarrow> 'v \<Rightarrow> bool" where
   "pcycle V E v0 \<equiv> \<exists>v\<in>V. (v0,v)\<in>E\<^sup>* \<and> (v,v)\<in>E\<^sup>+"
 (*for my purpose, it might be enough:
-  (x,x) \<notin> view^+ but this does not find undirected cycles! *)
+  \<forall> reachable v0 x. (x,x) \<notin> view^+ but this does not find undirected cycles! *)
 (*is basic routing loop detection*)
 
 
-definition acyclic :: "('v, 'v \<times> 'v) pre_digraph \<Rightarrow> bool" where
-  "acyclic G \<equiv> \<forall> u p v. pre_digraph.awalk G u p v \<longrightarrow> \<not> pre_digraph.cycle G p"
-
-lemma acyclic_alt: "wf_digraph G \<Longrightarrow> acyclic G = (\<forall> u \<in> verts G. \<forall> v \<in> verts G. \<forall> p. pre_digraph.awalk G u p v \<longrightarrow> \<not> pre_digraph.cycle G p)"
-  apply(simp add: acyclic_def wf_digraph_def)
-  by (metis (full_types) pre_digraph.awalk_def pre_digraph.cycle_def)
-
-lemma "\<not> acyclic \<lparr> pverts = {1::nat}, parcs = {(1,1)} \<rparr>"
-  apply(simp add: acyclic_def with_proj_def)
-  apply(rule_tac x="1" in exI)
-  apply(rule_tac x="[(1,1)]" in exI)
-  apply(rule conjI)
-  apply(rule_tac x="1" in exI)
-  apply(simp add: pre_digraph.awalk_def)
-  apply(simp add: pre_digraph.cas.simps)
-  apply(simp add: pre_digraph.cycle_def)
-  apply(simp add: pre_digraph.awalk_def)
-  apply(simp add: pre_digraph.cas.simps)
-  apply(simp add: pre_digraph.awalk_verts.simps)
-  done
-lemma "\<not> acyclic \<lparr> pverts = {1::nat,2,3}, parcs = {(1,2),(2,3),(3,1)} \<rparr>"
-  apply(simp add: acyclic_def with_proj_def)
-  apply(rule_tac x="1" in exI)
-  apply(rule_tac x="[(1,2),(2,3),(3,1)]" in exI)
-  apply(rule conjI)
-  apply(rule_tac x="1" in exI)
-  apply(simp add: pre_digraph.awalk_def)
-  apply(simp add: pre_digraph.cas.simps)
-  apply(simp add: pre_digraph.cycle_def)
-  apply(simp add: pre_digraph.awalk_def)
-  apply(simp add: pre_digraph.cas.simps)
-  apply(simp add: pre_digraph.awalk_verts.simps)
-  done
-lemma "acyclic \<lparr> pverts = {1::nat,2,3}, parcs = {(1,2),(2,3),(1,3)} \<rparr>"
-  apply(subgoal_tac "wf_digraph \<lparr> pverts = {1::nat,2,3}, parcs = {(1,2),(2,3),(1,3)} \<rparr>")
-  apply(unfold_locales, auto)
-  apply(simp add: acyclic_alt with_proj_def)
-  apply(thin_tac "wf_digraph ?x")
-  apply(auto)
-  oops (*need a methot to calculate awalks*)
-
 hide_const(open) succ (*my succ in my graph*)
 
-
-(*An undirected graph has a cycle if and only if a depth-first search (DFS) 
-  finds an edge that points to an already-visited vertex (a back edge) [wikipedia] *)
-(*need to trace edges!!*)
-
-(*http://www.geeksforgeeks.org/detect-cycle-undirected-graph/*)
-
-fun neighbors :: "('v \<times> 'v) list \<Rightarrow> 'v \<Rightarrow> 'v list" where
-  "neighbors E v = map (\<lambda> (_,y). y) (filter (\<lambda>(x,y). x=v) E)"
-
-declare neighbors.simps[simp del]
-
-lemma set_neighbors: "set (neighbors E v) = {y. (v,y) \<in> set E}"
-by (auto simp add: neighbors.simps)
-
-(* v0 \<Rightarrow> visited \<Rightarrow> parent \<Rightarrow> neighbors *)
-function x_cycle :: "'v \<Rightarrow> 'v list \<Rightarrow> 'v \<Rightarrow> (('v \<times> 'v) list) \<Rightarrow> bool" where
-  "x_cycle v visited parent E = ((neighbors E v \<noteq> []) \<and> (\<forall> nxt \<in> set (neighbors E v). (if nxt \<notin> set visited
-    then
-      x_cycle nxt (v#visited) v E
-    else
-      nxt \<noteq> parent)))"
-apply pat_completeness
-by auto
-
-(*how do I termination?*)
-termination x_cycle
-apply (relation "measure (\<lambda>(v,vis,p,E). Suc(length E) - length vis)")
-apply(simp)
-apply(simp only: set_neighbors)
-oops
-
-value "x_cycle (1::nat) [] 1 [(1,2), (2,3), (3,1)]"
-value "x_cycle (1::nat) [] 1 [(1,2), (2,3), (1,3)]"
-
-
-
-(*Tets with DFS AFP*)
-
-(*E should be a DAG, finds cycles in the underlying undirected graph
-*)
-(* E worklist visited*)
-function y_cycle :: "(('v \<times> 'v) list) \<Rightarrow> 'v list \<Rightarrow> 'v set \<Rightarrow> bool" where
-  "y_cycle E [] vis = False" |
-  "y_cycle E (w#ws) vis = (if w \<in> vis then True 
-                        else y_cycle E (neighbors E w@ws) (insert w vis))"
-by pat_completeness auto
-
-termination (*I HAVE NO IDEA how to do termination proofs ... Where is this documented?*)
-apply (relation "inv_image (finite_psubset <*lex*> less_than)  
-                   (\<lambda>(E,w,vis). ((fst ` set E \<union> snd ` set E) - vis, size w))")
-apply auto[1]
-apply (simp_all add: finite_psubset_def)
-apply(case_tac "w \<in> (fst ` set E \<union> snd ` set E)")
-apply(auto simp add: neighbors.simps)
-by (metis (lifting, mono_tags) filter_False imageI split_beta)
-
-
-value "y_cycle [(1,2), (2,3), (3,1)] [1::nat] {}"
-value "(1,1) \<in> {(1::nat,2::nat), (2,3), (3,1)}^+"
-value "y_cycle [(1,2), (2,3), (1,3)] [1::nat] {}"
-value "{(1::nat,2::nat), (2,3), (1,3)}^+"
-value "y_cycle [(1,2), (2,3), (3,4)] [1::nat] {}"
-value "y_cycle [(1,2), (2,1)] [1::nat] {}" (*not a DAG*)
-value "(1,1) \<in> {(1::nat,2::nat), (2,1)}^+"
-value "y_cycle [(1,1)] [1::nat] {}"
-value "y_cycle [(1,2), (1,3), (3,4), (1,5), (5,6), (2,4)] [1::nat] {}"
-
-
-
-(*
-How do I formalize that the underlying undirected graph is acyclic?
-Digraph.symmetric
-*)
-definition "underlying_undirected_cycle \<equiv> 
-\<exists>p u. awalk u p u \<and> distinct (tl (awalk_verts u p)) \<and> length p \<ge> 3"
-
-
-
-
-
-
-
-
-
-
+definition nodes_of :: "('v \<times> 'v) set \<Rightarrow> 'v set" where "nodes_of E \<equiv> (fst ` E \<union> snd ` E)"
 
 
 (*Collections&Refinement tests*)
 
 
-(*does this really detetc cycles?*)
+(*requires: no loops (x,x) \<in> E*)
 (*V=worklist, (vertex, parent)*)
-definition cycles_dfs_imp :: "('a \<Rightarrow>'a set) \<Rightarrow> 'a \<Rightarrow> bool nres" 
+definition cycles_dfs_imp :: "('a \<times>'a) set \<Rightarrow> 'a \<Rightarrow> bool nres" 
   where
-  "cycles_dfs_imp succ v0 \<equiv>  do {
-      (_,_,cycle) \<leftarrow> WHILE (\<lambda> (V,Discovered,cycle). V \<noteq> {} \<and> \<not> cycle) (\<lambda> (V,Discovered,cycle). do {
-        (v,vparent) \<leftarrow> SPEC (\<lambda>v. v\<in>V );
-        let succs = (succ v) - {vparent};
-        if succs \<inter> fst ` Discovered  \<noteq> {} then RETURN (V,Discovered,True) else do {
-          let V = V - {(v,vparent)};
-          let Discovered = insert (v,vparent) Discovered;
-          let V = V \<union> ((succ v) \<times> {v});
-          RETURN (V,Discovered,cycle)
+  "cycles_dfs_imp E v0 \<equiv>  do {
+      (_,_,cycle) \<leftarrow> WHILE (\<lambda> (W,Discovered,cycle). W \<noteq> {} \<and> \<not> cycle) (\<lambda> (W,Discovered,cycle). do {
+        (vparent,v) \<leftarrow> SPEC (\<lambda>v. v\<in>W);
+        if v \<in> snd ` Discovered
+        then
+          RETURN (W,Discovered,True)
+        else do {
+          let succs = {v'. (v,v')\<in>E \<or> (v',v)\<in>E} - {vparent,v}; (*exclude self-loops*)
+          let W = W - {(vparent,v)};
+          let Discovered = insert (vparent,v) Discovered;
+          let W = W \<union> ({v} \<times> succs);
+          RETURN (W,Discovered,cycle)
         }
       }) ({(v0,v0)},{},False);
       RETURN cycle
   }"
 
+lemma "\<lbrakk> x\<in>snd`D; y\<in>snd`D; x \<noteq> y\<rbrakk> \<Longrightarrow> (\<exists> p. set p \<subseteq> D \<and> pcas x p y)
+  \<longleftrightarrow>
+  (x,y) \<in> D\<^sup>+"
+apply(rule iffI)
+defer
+nitpick
+find_theorems intro
+oops
+
+
 (*everything reachable from V'*)
 lemma "{y. \<exists>x \<in> V'. (x,y) \<in> E\<^sup>*} = E\<^sup>*``V'" by blast
 
+definition restrict_to :: "('v \<times> 'v) set \<Rightarrow> 'v set \<Rightarrow> ('v \<times> 'v) set" where
+  "restrict_to E V \<equiv> {(a,b)\<in>E. a\<in>V \<and> b\<in>V}"
+
+definition bi :: "('a \<times> 'a) set \<Rightarrow> ('a \<times> 'a) set" where
+  "bi E = E \<union> backflows E"
+
+lemma bi_insert: "bi (insert (x,y) X) = {(x,y), (y,x)} \<union> bi X"
+  by(auto simp add: bi_def backflows_def)
+
+definition uni_restrict_to :: "('v \<times> 'v) set \<Rightarrow> 'v set \<Rightarrow> ('v \<times> 'v) set" where
+  "uni_restrict_to E V \<equiv> restrict_to (bi E) V"
+
+lemma uni_restrict_to_mono: "D' \<subseteq> D \<Longrightarrow> uni_restrict_to E D' \<subseteq> uni_restrict_to E D"
+  by(simp add: uni_restrict_to_def restrict_to_def, fast)
+
+
+
+definition has_undirected_cycle_in :: "('a \<times> 'a) set \<Rightarrow> bool" where
+  "has_undirected_cycle_in E \<equiv> 
+  \<exists> u \<in> nodes_of E. \<exists> p. set p \<subseteq> bi E \<and> pcas u p u \<and> distinct (tl (Pair_Digraph.pawalk_verts u p)) \<and> length p \<ge> 3"
+
+
 definition cycles_dfs_imp_WHILE_invar :: "('v \<times> 'v) set \<Rightarrow> 'v \<Rightarrow> ('v\<times>'v) set \<times> ('v\<times>'v) set \<times> bool \<Rightarrow> bool" where
-  "cycles_dfs_imp_WHILE_invar E v0 \<sigma> \<equiv> let (V',Discovered,cycle) = \<sigma> in
-        V' \<subseteq> insert (v0,v0) E \<and> Discovered \<subseteq> insert (v0,v0) E \<and> 
-        E\<^sup>*``(fst ` V') \<union> fst ` Discovered = E\<^sup>*``{v0} \<and> 
-        ( Discovered \<inter> V' = {})"
-        (*{(a,b) \<in> E. a \<in> Discovered \<and> b \<in> Discovered} = E*)
-        (*need condition: no cycle so far!*)
+  "cycles_dfs_imp_WHILE_invar E v0 \<sigma> \<equiv> let (W,D,cycle) = \<sigma> in
+        W \<subseteq> bi E \<and> D \<subseteq> bi E
+        \<and> (\<forall> (a,_) \<in> W. \<exists> (_,d) \<in> D. (d,a) \<in> D)
+        \<and> (\<forall> x\<in>snd`D. \<forall> y\<in>snd`D. x \<noteq> y \<longrightarrow> (x,y) \<in> (bi D)\<^sup>+)
+        \<and> (cycle \<longrightarrow> has_undirected_cycle_in (D \<union> W)) 
+        (*\<and> (\<forall> x\<in>Discovered. \<forall> y\<in>Discovered. x \<noteq> y \<longrightarrow> 
+            (\<exists> p. set p \<subseteq> uni_restrict_to E (Discovered) \<and> pcas x p y \<and> distinct (Pair_Digraph.pawalk_verts x p)))*)
+        (*E\<^sup>*``(fst ` V') \<union> fst ` Discovered = E\<^sup>*``{v0} \<and> *)"
 
 lemma cycles_dfs_imp_WHILE_invar_step1:
-  assumes "V = E\<^sup>*``{v0}" and "cycles_dfs_imp_WHILE_invar V E v0 (V',Discovered,cycle)"
-      "V' \<noteq> {}" "\<not> cycle" "x \<in> V'" "x \<in> Discovered"
-  shows "cycles_dfs_imp_WHILE_invar V E v0 (V', Discovered, True)"
-  using assms apply(simp add: cycles_dfs_imp_WHILE_invar_def) by blast
-
-lemma cycles_dfs_imp_WHILE_invar_step2:
-  assumes "V = E\<^sup>*``{v0}" and "cycles_dfs_imp_WHILE_invar V E v0 (V', Discovered, cycle)"
-       "V' \<noteq> {}" "\<not> cycle" "x \<in> V'" "x \<notin> Discovered"
-  shows "cycles_dfs_imp_WHILE_invar V E v0 (V' - {x} \<union> E `` {x}, insert x Discovered, cycle)"
-  using assms apply(simp add: cycles_dfs_imp_WHILE_invar_def)
-  apply(rule conjI)
-  apply blast
-  thm it_step_insert_iff
+  assumes "cycles_dfs_imp_WHILE_invar E v0 (W, Discovered, cycle)"
+       "(a, snd (d1, d2)) \<in> W" "(d1, d2) \<in> Discovered" "W \<noteq> {}" "\<not> cycle" 
+  shows "cycles_dfs_imp_WHILE_invar E v0 (W, Discovered, True)"
+  using assms unfolding cycles_dfs_imp_WHILE_invar_def
+  apply(simp)
+  (*TODO*)
 oops
 
-lemma cycles_dfs_imp_WHILE_invar_goal_c1: 
-  assumes "V = E\<^sup>*``{v0}" and "cycles_dfs_imp_WHILE_invar V E v0 ({},Discovered,cycle)"
-  shows "\<not> cycle \<longleftrightarrow> (\<forall>x\<in>V. (v0, x) \<in> E\<^sup>* \<longrightarrow> (x, x) \<notin> E\<^sup>+)"
-  using assms by(auto simp add: cycles_dfs_imp_WHILE_invar_def)
+lemma nodes_of_backflows_snd: "nodes_of E = snd ` E \<union> snd ` (backflows E)"
+    apply(simp add: nodes_of_def backflows_alt_fstsnd) by force
+lemma nodes_of_subset_backflows_b: "v0 \<in> nodes_of E \<Longrightarrow> V \<subseteq> insert (v0,v0) (E \<union> backflows E) \<Longrightarrow> (a, b) \<in> V \<Longrightarrow> b \<in> nodes_of E"
+    apply(simp add: nodes_of_backflows_snd) by force
+
+lemma "y \<in> snd ` (V - {(a, b)} \<union> {b} \<times> ({v'. (b, v') \<in> E \<or> (v', b) \<in> E} - {a, b})) \<Longrightarrow>
+         b \<noteq> y \<Longrightarrow>  y \<notin> snd ` V \<Longrightarrow> False" oops
+
+lemma cycles_dfs_imp_WHILE_invar_step2:
+  assumes "v0 \<in> nodes_of E" and "cycles_dfs_imp_WHILE_invar E v0 (W, Discovered, False)"
+       "(w1, w2) \<in> W"
+       "w2 \<notin> snd ` Discovered"
+       "W \<noteq> {}"
+       "\<not> cycle"
+  shows "cycles_dfs_imp_WHILE_invar E v0 (W - {(w1, w2)} \<union> {w2} \<times> ({v'. (w2, v') \<in> E \<or> (v', w2) \<in> E} - {w1, w2}), insert (w1, w2) Discovered, False)" 
+  using assms unfolding cycles_dfs_imp_WHILE_invar_def
+  apply(simp)
+  apply(rule conjI)
+  apply(auto)[1]
+  apply(rule conjI)
+  apply(auto simp add: bi_def backflows_def)[1]
+  apply(rule conjI)
+  apply(auto simp add: bi_def backflows_def)[1]
+  apply(rule conjI)
+  apply blast
+  apply(rule conjI)
+  apply(simp add: bi_insert)[1]
+  apply(clarsimp)
+  apply(erule_tac x="(w1,w2)" in ballE, simp)
+  prefer 2 apply simp
+  apply(erule bexE)
+  apply(clarify)
+  (*holds but needs proof ...*)
+    using nodes_of_subset_backflows_b
+oops
 
 lemma cycles_dfs_imp_sound:
   fixes succ and v0
-  defines "E \<equiv> {(v,v'). v'\<in>succ v}"
-  defines "V \<equiv> {v. (v0,v)\<in>E\<^sup>*}"
-  assumes F: "finite V"
-  shows "cycles_dfs_imp succ v0 \<le> SPEC (\<lambda>r. \<not> r \<longleftrightarrow> (\<forall>x\<in>V. (v0,x)\<in>E\<^sup>* \<longrightarrow> (x,x)\<notin>E\<^sup>+))"
+  assumes F: "finite E"
+  shows "cycles_dfs_imp E v0 \<le> SPEC (\<lambda>r. r \<longleftrightarrow> has_undirected_cycle_in (uni_restrict_to E (E\<^sup>*``{v0})))"
 proof -
-  have S: "\<And>v. succ v = E``{v}"
-    by (auto simp: E_def)
-  have V: "V = E\<^sup>*``{v0}"
-    by (auto simp: V_def)
   
   from F show ?thesis
-    unfolding cycles_dfs_imp_def S
+    unfolding cycles_dfs_imp_def
     apply(intro WHILE_rule[where I="cycles_dfs_imp_WHILE_invar E v0"] refine_vcg)
-    apply(auto simp add: V_def cycles_dfs_imp_WHILE_invar_def)[1]
-    apply(clarify)
-    apply(drule(5) cycles_dfs_imp_WHILE_invar_step1[OF V])
-    apply(clarify)
-    prefer 2
-    apply(simp add: cycles_dfs_imp_WHILE_invar_goal_c1)
-    apply(auto simp add: V_def cycles_dfs_imp_WHILE_invar_def)[1]
+    apply(auto simp add: cycles_dfs_imp_WHILE_invar_def restrict_to_def has_undirected_cycle_in_def nodes_of_def)[1]
+    apply(clarify, rename_tac A W C V Discovered cycle I J a L d1 d2)
+    apply(simp add: cycles_dfs_imp_WHILE_invar_step1)
+    apply(clarsimp)
+    apply(rename_tac W Discovered cycle w1 w2)
+    apply(auto simp add: cycles_dfs_imp_WHILE_invar_def)[1]
+    apply(simp add: cycles_dfs_imp_WHILE_invar_def)[1]
+    apply(rule conjI)
+    apply(auto)[1]
+    apply(rule conjI)
+    apply(auto)[1]
+    apply(rule conjI)
+    apply(auto)[1]
+    apply clarify
+    using v0 try0
     oops
 
-
-
-(**The old version***)
-definition cycles_dfs_imp_WHILE_invar :: "'v set \<Rightarrow> ('v \<times> 'v) set \<Rightarrow> 'v \<Rightarrow> 'v set \<times> 'v set \<times> bool \<Rightarrow> bool" where
-  "cycles_dfs_imp_WHILE_invar V E v0 \<sigma> \<equiv> let (V',Discovered,cycle) = \<sigma> in
-        V' \<subseteq> V \<and> Discovered \<subseteq> V \<and> 
-        (*E\<^sup>*``V' = V - Discovered *) (*Discovered = V - E\<^sup>*``V'*) E\<^sup>*``V' \<union> Discovered = V \<and> 
-        ( Discovered \<inter> V' = {}) \<and>
-        ( \<not>cycle \<longleftrightarrow> (\<forall>x\<in>Discovered. (v0, x) \<in> E\<^sup>* \<longrightarrow> (x,x)\<notin>E\<^sup>+))"
-        (*{(a,b) \<in> E. a \<in> Discovered \<and> b \<in> Discovered} = E*)
-        (*need condition: no cycle so far!*)
-
-lemma cycles_dfs_imp_WHILE_invar_step1:
-  assumes "V = E\<^sup>*``{v0}" and "cycles_dfs_imp_WHILE_invar V E v0 (V',Discovered,cycle)"
-      "V' \<noteq> {}" "\<not> cycle" "x \<in> V'" "x \<in> Discovered"
-  shows "cycles_dfs_imp_WHILE_invar V E v0 (V', Discovered, True)"
-  using assms apply(simp add: cycles_dfs_imp_WHILE_invar_def) by blast
-
-lemma cycles_dfs_imp_WHILE_invar_step2:
-  assumes "V = E\<^sup>*``{v0}" and "cycles_dfs_imp_WHILE_invar V E v0 (V', Discovered, cycle)"
-       "V' \<noteq> {}" "\<not> cycle" "x \<in> V'" "x \<notin> Discovered"
-  shows "cycles_dfs_imp_WHILE_invar V E v0 (V' - {x} \<union> E `` {x}, insert x Discovered, cycle)"
-  using assms apply(simp add: cycles_dfs_imp_WHILE_invar_def)
-  apply(rule conjI)
-  apply blast
-  apply(rule conjI)oops
-apply (metis Image_singleton_iff rtrancl.rtrancl_into_rtrancl subsetD subsetI)
-  apply(rule conjI)
-  apply blast
-  apply(rule conjI)
-apply (metis Un_insert_left insert_Diff_single insert_subset rtrancl_apply_insert subsetI subset_antisym)
-  apply(rule conjI)defer 
-  apply(rule conjI)
-  oops
-  apply(rule conjI)
-  thm it_step_insert_iff
-oops
-
-lemma cycles_dfs_imp_WHILE_invar_goal_c1: 
-  assumes "V = E\<^sup>*``{v0}" and "cycles_dfs_imp_WHILE_invar V E v0 ({},Discovered,cycle)"
-  shows "\<not> cycle \<longleftrightarrow> (\<forall>x\<in>V. (v0, x) \<in> E\<^sup>* \<longrightarrow> (x, x) \<notin> E\<^sup>+)"
-  using assms by(auto simp add: cycles_dfs_imp_WHILE_invar_def)
-
-lemma cycles_dfs_imp_sound:
-  fixes succ and v0
-  defines "E \<equiv> {(v,v'). v'\<in>succ v}"
-  defines "V \<equiv> {v. (v0,v)\<in>E\<^sup>*}"
-  assumes F: "finite V"
-  shows "cycles_dfs_imp succ v0 \<le> SPEC (\<lambda>r. \<not> r \<longleftrightarrow> (\<forall>x\<in>V. (v0,x)\<in>E\<^sup>* \<longrightarrow> (x,x)\<notin>E\<^sup>+))"
-proof -
-  have S: "\<And>v. succ v = E``{v}"
-    by (auto simp: E_def)
-  have V: "V = E\<^sup>*``{v0}"
-    by (auto simp: V_def)
-  
-  from F show ?thesis
-    unfolding cycles_dfs_imp_def S
-    apply(intro WHILE_rule[where I="cycles_dfs_imp_WHILE_invar V E v0"] refine_vcg)
-    apply(auto simp add: V_def cycles_dfs_imp_WHILE_invar_def)[1]
-    apply(clarify)
-    apply(drule(5) cycles_dfs_imp_WHILE_invar_step1[OF V])
-    apply(clarify)
-    prefer 2
-    apply(simp add: cycles_dfs_imp_WHILE_invar_goal_c1)
-    apply(auto simp add: V_def cycles_dfs_imp_WHILE_invar_def)[1]
-    oops
 
 
 
 
 (*no idea what's wrong here*)
-definition cycles_dfs_rec :: "('a \<Rightarrow>'a set) \<Rightarrow> 'a \<Rightarrow> bool nres" 
+definition cycles_dfs_recX :: "('a \<Rightarrow>'a set) \<Rightarrow> 'a \<Rightarrow> bool nres" 
   where
-  "cycles_dfs_rec succ v0 \<equiv> REC (\<lambda>D (V,v). 
+  "cycles_dfs_recX succ v0 \<equiv> REC (\<lambda>D (V,v). 
     if v \<in> V then RETURN True 
     else do {
       let V=insert v V;
@@ -329,44 +200,60 @@ lemma cycles_dfs_rec_sound:
   defines "E \<equiv> {(v,v'). v'\<in>succ v}"
   defines "V \<equiv> {v. (v0,v)\<in>E\<^sup>*}"
   assumes F: "finite V"
-  shows "cycles_dfs_rec succ v0 \<le> SPEC (\<lambda>r. r \<longrightarrow> (\<forall>x\<in>V. (v0,x)\<in>E\<^sup>* \<longrightarrow> (x,x)\<notin>E\<^sup>+))"
+  shows "cycles_dfs_recX succ v0 \<le> SPEC (\<lambda>r. r \<longrightarrow> (\<forall>x\<in>V. (v0,x)\<in>E\<^sup>* \<longrightarrow> (x,x)\<notin>E\<^sup>+))"
 proof -
   have S: "\<And>v. succ v = E``{v}"
     by (auto simp: E_def)
   
   from F show ?thesis
-    unfolding cycles_dfs_rec_def S
+    unfolding cycles_dfs_recX_def S
     apply(intro REC_rule[where \<Phi>="\<lambda>(V',v'). (v0,v')\<in>E\<^sup>* \<and> V'\<subseteq>V \<and> (\<forall>x\<in>V'. (v0,x)\<in>E\<^sup>* \<longrightarrow> (x,x)\<notin>E\<^sup>+)"] 
         FOREACH_rule[where I="\<lambda>Succs r. XXX"] refine_vcg) (*r \<longrightarrow> (\<forall>v\<in>V. (v0,v)\<in>E\<^sup>* \<longrightarrow> (v,v)\<notin>E\<^sup>+)*)
     apply(refine_mono) (*REC is somehow undocumented*)
     apply(simp)
     apply(simp_all)
     apply(rename_tac V' v')
-    apply(intro FOREACH_rule[where I="\<lambda>_ r. r \<longrightarrow> (\<forall>v\<in>V. (v0,v)\<in>E\<^sup>* \<longrightarrow> (v,v)\<notin>E\<^sup>+)"] refine_vcg)
-    apply(refine_rcg)
-    apply(auto)
-    apply(refine_rcg refine_vcg impI REC_rule[where 
-        \<Phi>="\<lambda>(V,v). (v0,v)\<in>E\<^sup>* \<and> V\<subseteq>{v. (v0,v)\<in>E\<^sup>*} \<and> \<not>(\<exists>v\<in>V. (v0,v)\<in>E\<^sup>* \<and> (v,v)\<in>E\<^sup>+)"]
-        FOREACH_rule[where I="\<lambda>_ r. r \<longrightarrow> (\<forall>v\<in>V. (v0,v)\<in>E\<^sup>* \<longrightarrow> (v,v)\<notin>E\<^sup>+)"])
-    apply(auto)
-    apply(auto simp add: acyclic_alt[OF wf_G])
-    (*apply (refine_rcg refine_vcg impI
-      RECT_rule[where 
-        \<Phi>="\<lambda>(V,v). (v0,v)\<in>E\<^sup>* \<and> V\<subseteq>{v. (v0,v)\<in>E\<^sup>*}" and
-        V="finite_psupset ({v. (v0,v)\<in>E\<^sup>*}) <*lex*> {}"]
-      FOREACHc_rule[where I="\<lambda>_ r. r \<longrightarrow> (v0, vd) \<in> E\<^sup>*"]
-    )*)
+    oops
+
+
+
+
+
+
+
+
+
+
+fun fibdef :: "nat \<Rightarrow> nat" where
+  "fibdef 0 = 1" |
+  "fibdef (Suc 0) = 1" |
+  "fibdef (Suc (Suc n)) = fibdef (Suc n) + fibdef n"
+value "fibdef 4"
+
+definition fibref :: "nat \<Rightarrow> nat nres" 
+  where
+  "fibref n \<equiv> REC (\<lambda>D (n). 
+    if n = 0 then RETURN 1
+    else if n = 1 then RETURN 1
+    else do { 
+      x \<leftarrow> (D (n - 1));
+      y \<leftarrow> (D (n - 2));
+      RETURN (x + y)
+      }
+    ) (n)"
+
+lemma fibref:
+  shows "fibref n \<le> SPEC (\<lambda>r. r = fibdef n)"
+proof -
+  show ?thesis
+    unfolding fibref_def
+    apply (refine_rcg refine_vcg REC_rule[where \<Phi>="\<lambda>n. n \<ge> 0"])
+    apply(simp_all)[3]
+    apply(simp add: RETURN_def)
     apply(auto)
     oops
 
-(*TODO only acyclic in reachable from v0*)
 
-
-
-
-section{*cycles*}
-(*An undirected graph has a cycle if and only if a depth-first search (DFS) 
-  finds an edge that points to an already-visited vertex (a back edge) [wikipedia] *)
 
 
 section{*TEST TEST TES TEST of UNIO*}
